fork be gone. iris_meta broken

core_lang.v
@@ -12,20 +12,20 @@ Module Type CORE_LANG.
   Parameter is_value_dec : forall e, is_value e + ~is_value e.
 
   (* fork and fRet *)
-  Parameter fork : expr -> expr.
-  Parameter fork_ret : expr.
-  Axiom fork_ret_is_value : is_value fork_ret.
-  Definition fork_ret_val : value := exist _ fork_ret fork_ret_is_value.
-  Axiom fork_not_value : forall e,
-                           ~is_value (fork e).
-  Axiom fork_inj : forall e1 e2,
-                     fork e1 = fork e2 -> e1 = e2.
+  (* Parameter fork : expr -> expr. *)
+  (* Parameter fork_ret : expr. *)
+  (* Axiom fork_ret_is_value : is_value fork_ret. *)
+  (* Definition fork_ret_val : value := exist _ fork_ret fork_ret_is_value. *)
+  (* Axiom fork_not_value : forall e, *)
+  (*                          ~is_value (fork e). *)
+  (* Axiom fork_inj : forall e1 e2, *)
+  (*                    fork e1 = fork e2 -> e1 = e2. *)
 
   (** Evaluation contexts **)
-  Parameter ectx : Type.
-  Parameter empty_ctx : ectx.
-  Parameter comp_ctx : ectx -> ectx -> ectx.
-  Parameter fill : ectx -> expr -> expr.
+  (* Parameter ectx : Type. *)
+  (* Parameter empty_ctx : ectx. *)
+  (* Parameter comp_ctx : ectx -> ectx -> ectx. *)
+  (* Parameter fill : ectx -> expr -> expr. *)
 (*
 	All of
 		comp_ctx_assoc
@@ -50,20 +50,20 @@ Module Type CORE_LANG.
 	It might be simpler to (prove and) assume these two rather
 	than those four.
 *)
-  Axiom comp_ctx_emp_r : forall K,
-    comp_ctx K empty_ctx = K.
-  Axiom comp_ctx_assoc : forall K0 K1 K2,
-    comp_ctx K0 (comp_ctx K1 K2) = comp_ctx (comp_ctx K0 K1) K2.
-  Axiom comp_ctx_inj_r : forall K K1 K2,
-    comp_ctx K K1 = comp_ctx K K2 -> K1 = K2.
-  Axiom comp_ctx_positive : forall K1 K2,
-    comp_ctx K1 K2 = empty_ctx -> K1 = empty_ctx /\ K2 = empty_ctx.
+  (* Axiom comp_ctx_emp_r : forall K, *)
+  (*   comp_ctx K empty_ctx = K. *)
+  (* Axiom comp_ctx_assoc : forall K0 K1 K2, *)
+  (*   comp_ctx K0 (comp_ctx K1 K2) = comp_ctx (comp_ctx K0 K1) K2. *)
+  (* Axiom comp_ctx_inj_r : forall K K1 K2, *)
+  (*   comp_ctx K K1 = comp_ctx K K2 -> K1 = K2. *)
+  (* Axiom comp_ctx_positive : forall K1 K2, *)
+  (*   comp_ctx K1 K2 = empty_ctx -> K1 = empty_ctx /\ K2 = empty_ctx. *)
 
-  Axiom fill_empty : forall e, fill empty_ctx e = e.
-  Axiom fill_comp  : forall K1 K2 e, fill K1 (fill K2 e) = fill (comp_ctx K1 K2) e.
-  Axiom fill_inj_r  : forall K e1 e2, fill K e1 = fill K e2 -> e1 = e2.
-  Axiom fill_value : forall K e, is_value (fill K e) -> is_value e.
-  Axiom fill_fork : forall K e e', fork e' = fill K e -> K = empty_ctx.
+  (* Axiom fill_empty : forall e, fill empty_ctx e = e. *)
+  (* Axiom fill_comp  : forall K1 K2 e, fill K1 (fill K2 e) = fill (comp_ctx K1 K2) e. *)
+  (* Axiom fill_inj_r  : forall K e1 e2, fill K e1 = fill K e2 -> e1 = e2. *)
+  (* Axiom fill_value : forall K e, is_value (fill K e) -> is_value e. *)
+  (* Axiom fill_fork : forall K e e', fork e' = fill K e -> K = empty_ctx. *)
 
   (** Shared machine state (e.g., the heap) **)
   Parameter state : Type.
@@ -71,20 +71,19 @@ Module Type CORE_LANG.
   (** Primitive (single thread) machine configurations **)
   Definition prim_cfg : Type := (expr * state)%type.
 
+  Definition thread_id := nat.
+  
   (** The primitive atomic stepping relation **)
-  Parameter prim_step : prim_cfg -> prim_cfg -> Prop.
-
+  Parameter prim_step : prim_cfg -> prim_cfg -> option expr -> Prop.
 
   Definition reducible e: Prop :=
-    exists sigma cfg', prim_step (e, sigma) cfg'.
+    exists sigma cfg' oe, prim_step (e, sigma) cfg' oe.
 
   Definition stuck (e : expr) : Prop :=
-    forall K e',
-      e = fill K e' ->
-      ~reducible e'.
+      ~reducible e.
 
-  Axiom fork_stuck :
-    forall K e, stuck (fill K (fork e) ).
+  (* Axiom fork_stuck : *)
+  (*   forall K e, stuck (fill K (fork e) ). *)
   Axiom values_stuck :
     forall e, is_value e -> stuck e.
 
@@ -92,19 +91,19 @@ Module Type CORE_LANG.
      expression has a non-value e in the hole, then K is a left
      sub-context of K' - in other words, e also contains the reducible
      expression *)
-  Axiom step_by_value :
-    forall K K' e e',
-      fill K e = fill K' e' ->
-      reducible e' ->
-      ~ is_value e ->
-      exists K'', K' = comp_ctx K K''.
-  (* Similar to above, buth with a fork instead of a reducible
-     expression *)
-  Axiom fork_by_value :
-    forall K K' e e',
-      fill K e = fill K' (fork e') ->
-      ~ is_value e ->
-      exists K'', K' = comp_ctx K K''.
+  (* Axiom step_by_value : *)
+  (*   forall K K' e e', *)
+  (*     fill K e = fill K' e' -> *)
+  (*     reducible e' -> *)
+  (*     ~ is_value e -> *)
+  (*     exists K'', K' = comp_ctx K K''. *)
+  (* (* Similar to above, buth with a fork instead of a reducible *)
+  (*    expression *) *)
+  (* Axiom fork_by_value : *)
+  (*   forall K K' e e', *)
+  (*     fill K e = fill K' (fork e') -> *)
+  (*     ~ is_value e -> *)
+  (*     exists K'', K' = comp_ctx K K''. *)
 
   (** Atomic expressions **)
   Parameter atomic : expr -> Prop.
@@ -112,9 +111,9 @@ Module Type CORE_LANG.
   Axiom atomic_reducible :
     forall e, atomic e -> reducible e.
 
-  Axiom atomic_step: forall e σ e' σ',
+  Axiom atomic_step: forall e σ e' σ' oe,
                        atomic e ->
-                       prim_step (e, σ) (e', σ') ->
+                       prim_step (e, σ) (e', σ') oe ->
                        is_value e'.
 
 End CORE_LANG.
