lang.v
@@ -16,18 +16,18 @@ Module Lang (C : CORE_LANG).
   Delimit Scope lang_scope with lang.
   Local Open Scope lang_scope.
 
-  Notation "'ε'"    := empty_ctx : lang_scope.
-  Notation "K1 ∘ K2"  := (comp_ctx K1 K2) (at level 40, left associativity) : lang_scope.
+  (* Notation "'ε'"    := empty_ctx : lang_scope. *)
+  (* Notation "K1 ∘ K2"  := (comp_ctx K1 K2) (at level 40, left associativity) : lang_scope. *)
 
-  Arguments fork_not_value {_} _.
-  Arguments comp_ctx_positive {_ _} _.
-  Arguments fork_inj {_ _} _.
-  Arguments fill_inj_r _ {_ _} _.
-  Arguments fill_value {_ _} _.
-  Arguments fill_fork {_ _ _} _.
-  Arguments values_stuck {_} _ {_ _} _ _.
-  Arguments atomic_reducible {_} _.
-  Arguments atomic_step {_ _ _ _} _ _.
+  (* Arguments fork_not_value {_} _. *)
+  (* Arguments comp_ctx_positive {_ _} _. *)
+  (* Arguments fork_inj {_ _} _. *)
+  (* Arguments fill_inj_r _ {_ _} _. *)
+  (* Arguments fill_value {_ _} _. *)
+  (* Arguments fill_fork {_ _ _} _. *)
+  (* Arguments values_stuck {_} _ {_ _} _ _. *)
+  (* Arguments atomic_reducible {_} _. *)
+  Arguments atomic_step {_ _ _ _} _ _ _.
 
   Local Open Scope lang_scope.
 
@@ -39,25 +39,32 @@ Module Lang (C : CORE_LANG).
 
   (* Threadpool stepping relation *)
   Inductive step (ρ ρ' : cfg) : Prop :=
-  | step_atomic : forall e e' σ σ' K t1 t2,
-      prim_step (e, σ) (e', σ') ->
-      ρ  = (t1 ++ fill K e  :: t2, σ) ->
-      ρ' = (t1 ++ fill K e' :: t2, σ') ->
+  | step_atomic : forall e e' σ σ' t1 t2,
+                    ρ  = (t1 ++ e  :: t2, σ) ->
+                    ρ' = (t1 ++ e' :: t2, σ') ->
+                    prim_step (e, σ) (e', σ') None ->
+                    step ρ ρ'
+  | step_atomic_fork : forall e e' σ σ' t1 t2 ef,
+                         ρ  = (t1 ++ e :: t2, σ) ->
+                         ρ' = (t1 ++ e' :: t2 ++ ef :: nil, σ') ->
+                         prim_step (e, σ) (e', σ') (Some ef) ->
       step ρ ρ'
-  | step_fork : forall e σ K t1 t2,
-      (* thread ID is 0 for the head of the list, new thread gets first free ID *)
-      ρ  = (t1 ++ fill K (fork e) :: t2, σ) ->
-      ρ' = (t1 ++ fill K fork_ret :: t2 ++ e :: nil, σ) ->
-      step ρ ρ'.
+  .
+  
+  (* | step_fork : forall e σ K t1 t2, *)
+  (*     (* thread ID is 0 for the head of the list, new thread gets first free ID *) *)
+  (*     ρ  = (t1 ++ fill K (fork e) :: t2, σ) -> *)
+  (*     ρ' = (t1 ++ fill K fork_ret :: t2 ++ e :: nil, σ) -> *)
+  (*     step ρ ρ'. *)
 
-  Lemma comp_ctx_neut_emp_r {K K'} :
-    K = K ∘ K' ->
-    K' = ε.
-  Proof.
-    intros HEq.
-    rewrite <- comp_ctx_emp_r in HEq at 1.
-    apply comp_ctx_inj_r in HEq; now symmetry.
-  Qed.
+  (* Lemma comp_ctx_neut_emp_r {K K'} : *)
+  (*   K = K ∘ K' -> *)
+  (*   K' = ε. *)
+  (* Proof. *)
+  (*   intros HEq. *)
+  (*   rewrite <- comp_ctx_emp_r in HEq at 1. *)
+  (*   apply comp_ctx_inj_r in HEq; now symmetry. *)
+  (* Qed. *)
 
   (* Lemmas about expressions *)
   Lemma reducible_not_value {e} :
@@ -65,57 +72,55 @@ Module Lang (C : CORE_LANG).
   Proof.
     intros H_red H_val.
     eapply values_stuck; try eassumption.
-    now erewrite fill_empty.
   Qed.
 
-  Lemma reducible_not_fork {e K e'} :
-    reducible e -> e <> fill K (fork e').
-  Proof.
-    move=> HRed HDec.
-    move: (fork_stuck K e'); rewrite -HDec -(fill_empty e) => HStuck {HDec}.
-    exact: (HStuck _ _ eq_refl).
-  Qed.
+  (* Lemma reducible_not_fork {e K e'} : *)
+  (*   reducible e -> e <> fill K (fork e'). *)
+  (* Proof. *)
+  (*   move=> HRed HDec. *)
+  (*   move: (fork_stuck K e'); rewrite -HDec -(fill_empty e) => HStuck {HDec}. *)
+  (*   exact: (HStuck _ _ eq_refl). *)
+  (* Qed. *)
 
-  Lemma step_same_ctx {K K' e e'} :
-                         fill K e = fill K' e' ->
-                         reducible e  ->
-                         reducible e' ->
-                         K = K'.
-  Proof.
-    intros H_fill H_red H_red'.
-    edestruct (step_by_value K K' e e') as [K'' H_K''].
-    - assumption.
-    - assumption.
-    - now apply reducible_not_value.
-    - edestruct (step_by_value K' K e' e) as [K''' H_K'''].
-      + now symmetry.
-      + assumption.
-      + now apply reducible_not_value.
-      + subst K.
-        rewrite <- comp_ctx_assoc in H_K''.
-        assert (H_emp := comp_ctx_neut_emp_r H_K'').
-        apply comp_ctx_positive in H_emp.
-        destruct H_emp as[H_K'''_emp H_K''_emp].
-        subst K'' K'''.
-        now rewrite comp_ctx_emp_r.
-  Qed.
+  (* Lemma step_same_ctx {K K' e e'} : *)
+  (*                        fill K e = fill K' e' -> *)
+  (*                        reducible e  -> *)
+  (*                        reducible e' -> *)
+  (*                        K = K'. *)
+  (* Proof. *)
+  (*   intros H_fill H_red H_red'. *)
+  (*   edestruct (step_by_value K K' e e') as [K'' H_K'']. *)
+  (*   - assumption. *)
+  (*   - assumption. *)
+  (*   - now apply reducible_not_value. *)
+  (*   - edestruct (step_by_value K' K e' e) as [K''' H_K''']. *)
+  (*     + now symmetry. *)
+  (*     + assumption. *)
+  (*     + now apply reducible_not_value. *)
+  (*     + subst K. *)
+  (*       rewrite <- comp_ctx_assoc in H_K''. *)
+  (*       assert (H_emp := comp_ctx_neut_emp_r H_K''). *)
+  (*       apply comp_ctx_positive in H_emp. *)
+  (*       destruct H_emp as[H_K'''_emp H_K''_emp]. *)
+  (*       subst K'' K'''. *)
+  (*       now rewrite comp_ctx_emp_r. *)
+  (* Qed. *)
 
   Lemma atomic_not_stuck {e} :
     atomic e -> ~stuck e.
   Proof.
     intros H_atomic H_stuck.
     eapply H_stuck.
-    - now erewrite fill_empty.
-    - now eapply atomic_reducible.
+    now eapply atomic_reducible.
   Qed.
 
-  Lemma fork_not_atomic K e :
-    ~atomic (fill K (fork e)).
-  Proof.
-    intros HAt.
-    apply atomic_not_stuck in HAt.
-    apply HAt, fork_stuck.
-  Qed.
+  (* Lemma fork_not_atomic K e : *)
+  (*   ~atomic (fill K (fork e)). *)
+  (* Proof. *)
+  (*   intros HAt. *)
+  (*   apply atomic_not_stuck in HAt. *)
+  (*   apply HAt, fork_stuck. *)
+  (* Qed. *)
 
   Lemma atomic_not_value e :
     atomic e -> ~is_value e.
@@ -125,17 +130,17 @@ Module Lang (C : CORE_LANG).
     tauto.
   Qed.
 
-  Lemma atomic_fill {e K}
-        (HAt : atomic (fill K e))
-        (HNV : ~ is_value e) :
-    K = empty_ctx.
-  Proof.
-    destruct (step_by_value K ε e (fill K e)) as [K' EQK].
-    - now rewrite fill_empty.
-    - now apply atomic_reducible.
-    - assumption.
-    - symmetry in EQK; now apply comp_ctx_positive in EQK.
-  Qed.
+  (* Lemma atomic_fill {e K} *)
+  (*       (HAt : atomic (fill K e)) *)
+  (*       (HNV : ~ is_value e) : *)
+  (*   K = empty_ctx. *)
+  (* Proof. *)
+  (*   destruct (step_by_value K ε e (fill K e)) as [K' EQK]. *)
+  (*   - now rewrite fill_empty. *)
+  (*   - now apply atomic_reducible. *)
+  (*   - assumption. *)
+  (*   - symmetry in EQK; now apply comp_ctx_positive in EQK. *)
+  (* Qed. *)
 
   (* Reflexive, transitive closure of the step relation *)
   Global Instance cfg_type : Setoid cfg := discreteType.
